



Identify the rate of change for each equation.

Answers

1) $y = -\frac{2}{6}x + 6$

1. _____

2) $y = \frac{6}{-10}x + 9$

2. _____

3) $y = \frac{2}{10}x - 9$

3. _____

4) $y = \frac{8}{-10}x - 3$

4. _____

5) $y = -\frac{1}{-8}x + 6$

5. _____

6) $y = \frac{9}{10}x + 0$

6. _____

7) $y = \frac{3}{-9}x + 10$

7. _____

8) $y = -1x - 8$

8. _____

9) $y = \frac{5}{6}x - 4$

9. _____

10) $y = \frac{2}{6}x - 1$

10. _____

11) $y = \frac{7}{-9}x + 6$

11. _____

12) $y = -\frac{2}{-3}x + 7$

12. _____

13) $y = -5x + 2$

13. _____

14) $y = \frac{7}{-3}x + 8$

14. _____

15) $y = -3x + 1$

15. _____

16) $y = -\frac{9}{-8}x - 8$

16. _____

17) $y = \frac{3}{5}x + 5$

17. _____

18) $y = 8x + 7$

18. _____

19) $y = -8x + 7$

19. _____



Identify the rate of change for each equation.

Answers

- 1) $y = -\frac{2}{6}x + 6$
- 2) $y = \frac{6}{-10}x + 9$
- 3) $y = \frac{2}{10}x - 9$
- 4) $y = \frac{8}{-10}x - 3$
- 5) $y = -\frac{1}{-8}x + 6$
- 6) $y = \frac{9}{10}x + 0$
- 7) $y = \frac{3}{-9}x + 10$
- 8) $y = -1x - 8$
- 9) $y = \frac{5}{6}x - 4$
- 10) $y = \frac{2}{6}x - 1$
- 11) $y = \frac{7}{-9}x + 6$
- 12) $y = -\frac{2}{-3}x + 7$
- 13) $y = -5x + 2$
- 14) $y = \frac{7}{-3}x + 8$
- 15) $y = -3x + 1$
- 16) $y = -\frac{9}{-8}x - 8$
- 17) $y = \frac{3}{5}x + 5$
- 18) $y = 8x + 7$
- 19) $y = -8x + 7$

1. $|\frac{-2}{6}|$
2. $|\frac{6}{-10}|$
3. $|\frac{2}{10}|$
4. $|\frac{8}{-10}|$
5. $|\frac{-1}{-8}|$
6. $|\frac{9}{10}|$
7. $|\frac{3}{-9}|$
8. $|-1|$
9. $|\frac{5}{6}|$
10. $|\frac{2}{6}|$
11. $|\frac{7}{-9}|$
12. $|\frac{-2}{-3}|$
13. $|-5|$
14. $|\frac{7}{-3}|$
15. $|-3|$
16. $|\frac{-9}{-8}|$
17. $|\frac{3}{5}|$
18. $|8|$
19. $|-8|$